Setlec/SetP/ProjConsP.lean
@@ -247,6 +247,7 @@ theorem projConsP {env' : Env} (mp : EnvS2PM V μ env')
         (fun ψ => by rw [hAdef]; exact mp.base2.cval_closedL _ ψ)
         hnres (fun _ heq => by rw [hc₀] at heq; exact nomatch heq)
         (fun _ _ heq => by rw [hc₀] at heq; exact nomatch heq)
+        (fun _ heq => by rw [hc₀] at heq; exact nomatch heq)
         hctorsHead)
       hAclosedH hAparamsH
       (fun ψ ρ => by rw [hAdef]; exact mp.base2.acval_ok2 _ _ _)
